src/Lustre/Normalization/Fresh.v
@@ -9,196 +9,423 @@ From Velus Require Import Common Ident.
 
 (** The fresh monad (with memory) : generates new names and keeps
     a record of each name generated along with some information *)
-Definition fresh_st (B : Type) : Type := (ident * list (ident * B)).
-Definition Fresh (A B : Type) : Type := fresh_st B -> A * fresh_st B.
+Module Type FRESH.
 
-(** Pure value *)
-Definition ret {A B} (a : A) : Fresh A B := fun st => (a, st).
+  Section st.
+    Parameter fresh_st : Type -> Type.
+    Context {B : Type}.
+    Parameter st_anns : fresh_st B -> list (ident * B).
+    Definition st_ids (st : fresh_st B) := map fst (st_anns st).
+  End st.
 
-Section validity.
-  Context {B : Type}.
+  Definition Fresh (A B : Type) : Type := fresh_st B -> A * fresh_st B.
 
-  (** The state is valid if the next ident is greater than all generated idents,
-    and if there is no duplicates in generated idents *)
-  Definition fresh_st_valid (st : fresh_st B) : Prop :=
-    let '(n, l) := st in
-    Forall (fun '(x, _) => Pos.lt x n) l /\ NoDupMembers l.
-End validity.
+  Section ret.
+    Context {A B : Type}.
+    Parameter ret : A -> Fresh A B.
+    Axiom ret_spec : forall a st,
+        ret a st = (a, st).
+  End ret.
 
-Section follows.
-  Context {B : Type}.
+  Section validity.
+    Context {B : Type}.
+    Parameter fresh_st_valid : fresh_st B -> Prop.
+    Axiom st_valid_NoDupMembers : forall st,
+        fresh_st_valid st ->
+        NoDupMembers (st_anns st).
+  End validity.
 
-  (** Smallest identifier defined in the state *)
-  Definition smallest_ident (st : fresh_st B) : positive :=
-    let (n, l) := st in
-    fold_right Pos.min n (List.map fst l).
+  Section follows.
+    Context {B : Type}.
+    Parameter smallest_ident : fresh_st B -> ident.
+    Axiom smallest_ident_In : forall st x,
+        In x (st_ids st) ->
+        Pos.le (smallest_ident st) x.
+    Parameter fresh_st_follows : fresh_st B -> fresh_st B -> Prop.
+    Axiom st_follows_refl : Reflexive fresh_st_follows.
+    Axiom st_follows_trans : Transitive fresh_st_follows.
+    Axiom st_follows_smallest : forall st st',
+        fresh_st_follows st st' ->
+        Pos.le (smallest_ident st) (smallest_ident st').
+    Axiom st_follows_incl : forall st st',
+        fresh_st_follows st st' ->
+        incl (st_anns st) (st_anns st').
+  End follows.
 
-  (** The smallest ident of `st` is less or equal to the smallest
+  Section init.
+    Context {B : Type}.
+    Parameter init_st : ident -> fresh_st B.
+    Axiom init_st_anns : forall id, st_anns (init_st id) = [].
+    Axiom init_st_valid : forall id, fresh_st_valid (init_st id).
+    Axiom init_st_follows : forall id st',
+        fresh_st_follows (init_st id) st' ->
+        Forall (fun id' => Pos.le id id') (st_ids st').
+    Axiom init_st_smallest : forall id,
+        smallest_ident (init_st id) = id.
+  End init.
+
+  Section fresh_ident.
+    Context {B : Type}.
+    Parameter fresh_ident : B -> Fresh ident B.
+
+    Axiom fresh_ident_anns : forall b id st st',
+        fresh_ident b st = (id, st') ->
+        st_anns st' = (id, b)::(st_anns st).
+
+    Axiom fresh_ident_st_valid : forall b id st st',
+        fresh_ident b st = (id, st') ->
+        fresh_st_valid st ->
+        fresh_st_valid st'.
+    Axiom fresh_ident_st_follows : forall b id st st',
+        fresh_ident b st = (id, st') ->
+        fresh_st_follows st st'.
+    End fresh_ident.
+
+  Section bind.
+    Context {A A' B : Type}.
+    Parameter bind : Fresh A B -> (A -> Fresh A' B) -> Fresh A' B.
+    Axiom bind_spec : forall (x : Fresh A B) (k : A -> Fresh A' B) st a' st'',
+        (bind x k) st = (a', st'') <->
+        exists a, exists st', (x st = (a, st') /\ k a st' = (a', st'')).
+  End bind.
+
+  Section bind2.
+    Context {A1 A2 A' B : Type}.
+    Parameter bind2 : Fresh (A1 * A2) B -> (A1 -> A2 -> Fresh A' B) -> Fresh A' B.
+    Axiom bind2_spec : forall (x : Fresh (A1 * A2) B) (k : A1 -> A2 -> Fresh A' B) st a' st'',
+        (bind2 x k) st = (a', st'') <->
+        exists a1, exists a2, exists st', (x st = ((a1, a2), st') /\ k a1 a2 st' = (a', st'')).
+  End bind2.
+End FRESH.
+
+Module Fresh : FRESH.
+  Section st.
+    Definition fresh_st (B : Type) : Type := (ident * list (ident * B)).
+    Context {B : Type}.
+    Definition st_anns (st : fresh_st B) := snd st.
+    Definition st_ids (st : fresh_st B) := map fst (st_anns st).
+  End st.
+
+  Definition Fresh (A B : Type) : Type := fresh_st B -> A * fresh_st B.
+
+  Section ret.
+    Context {A B : Type}.
+    Definition ret (a : A) : Fresh A B := fun st => (a, st).
+
+    Fact ret_spec : forall a st,
+        ret a st = (a, st).
+    Proof.
+      intros a st. reflexivity.
+    Qed.
+  End ret.
+
+  Section validity.
+    Context {B : Type}.
+    (** The state is valid if the next ident is greater than all generated idents,
+        and if there is no duplicates in generated idents *)
+    Definition fresh_st_valid (st : fresh_st B) : Prop :=
+      let '(n, l) := st in
+      Forall (fun '(x, _) => Pos.lt x n) l /\ NoDupMembers l.
+
+    Fact st_valid_NoDupMembers : forall st,
+        fresh_st_valid st ->
+        NoDupMembers (st_anns st).
+    Proof.
+      intros st Hfresh.
+      destruct st; simpl in *.
+      destruct Hfresh. assumption.
+    Qed.
+  End validity.
+
+  Section follows.
+    Context {B : Type}.
+    (** Smallest identifier defined in the state *)
+    Definition smallest_ident (st : fresh_st B) : positive :=
+      let (n, l) := st in
+      fold_right Pos.min n (List.map fst l).
+
+    Fact smallest_ident_In : forall st x,
+        In x (st_ids st) ->
+        Pos.le (smallest_ident st) x.
+    Proof.
+      intros [n l] x Hin; simpl in *.
+      unfold st_ids in Hin; simpl in Hin.
+      eapply min_fold_in in Hin. eauto.
+    Qed.
+
+    (** The smallest ident of `st` is less or equal to the smallest
       ident of `st'` *)
-  Definition fresh_st_follows (st st' : fresh_st B) :=
-    incl (snd st) (snd st') /\
-    Pos.le (smallest_ident st) (smallest_ident st').
+    Definition fresh_st_follows (st st' : fresh_st B) :=
+      incl (snd st) (snd st') /\
+      Pos.le (smallest_ident st) (smallest_ident st').
 
-  Global Instance st_follows_refl : Reflexive fresh_st_follows.
-  Proof.
-    intros st. unfold fresh_st_follows.
-    split; reflexivity.
-  Qed.
+    Fact st_follows_refl : Reflexive fresh_st_follows.
+    Proof.
+      intros st. unfold fresh_st_follows.
+      split; reflexivity.
+    Qed.
 
-  Global Instance st_follows_trans : Transitive fresh_st_follows.
-  Proof.
-    unfold Transitive. intros.
-    unfold fresh_st_follows in *.
-    destruct H; destruct H0.
-    split; etransitivity; eauto.
-  Qed.
-End follows.
+    Fact st_follows_trans : Transitive fresh_st_follows.
+    Proof.
+      unfold Transitive. intros.
+      unfold fresh_st_follows in *.
+      destruct H; destruct H0.
+      split; etransitivity; eauto.
+    Qed.
 
-Section fresh_ident.
+    Fact st_follows_smallest : forall st st',
+        fresh_st_follows st st' ->
+        Pos.le (smallest_ident st) (smallest_ident st').
+    Proof.
+      intros st st' Hfollows.
+      destruct Hfollows. assumption.
+    Qed.
+
+    Fact st_follows_incl : forall st st',
+        fresh_st_follows st st' ->
+        incl (st_anns st) (st_anns st').
+    Proof.
+      intros st st' Hfollows.
+      destruct Hfollows. assumption.
+    Qed.
+  End follows.
+
+  Section init.
+    Context {B : Type}.
+
+    Definition init_st ident : fresh_st B := (ident, []).
+
+    Fact init_st_anns : forall id, st_anns (init_st id) = [].
+    Proof. intros. reflexivity.
+    Qed.
+
+    Fact init_st_valid : forall id, fresh_st_valid (init_st id).
+    Proof. intros id. unfold init_st. repeat constructor.
+    Qed.
+
+    Fact init_st_follows : forall id st',
+        fresh_st_follows (init_st id) st' ->
+        Forall (fun id' => Pos.le id id') (st_ids st').
+    Proof.
+      intros id st' Hfollows.
+      unfold init_st in Hfollows.
+      destruct Hfollows as [_ Hle]. destruct st'. simpl in *.
+      rewrite Forall_forall. intros x HIn. unfold st_ids in HIn. simpl in HIn.
+      eapply min_fold_in in HIn.
+      etransitivity; eauto.
+    Qed.
+
+    Fact init_st_smallest : forall id,
+        smallest_ident (init_st id) = id.
+    Proof.
+      intros id. reflexivity.
+    Qed.
+  End init.
+
+  Section fresh_ident.
+    Context {B : Type}.
+
+    Definition fresh_ident (b : B) : Fresh ident B :=
+      fun '(n, l) => (n, (Pos.succ n, (cons (n, b) l))).
+
+    Fact fresh_ident_anns : forall b id st st',
+        fresh_ident b st = (id, st') ->
+        st_anns st' = (id, b)::(st_anns st).
+    Proof.
+      intros.
+      destruct st. inv H.
+      reflexivity.
+    Qed.
+
+    Fact fresh_ident_st_valid :
+      forall (b : B) id st st',
+        fresh_ident b st = (id, st') ->
+        fresh_st_valid st ->
+        fresh_st_valid st'.
+    Proof.
+      intros b res st st' Hfresh Hvalid.
+      destruct st as [n l]; destruct st' as [n' l'].
+      simpl in Hfresh; inv Hfresh.
+      destruct Hvalid.
+      repeat constructor; auto.
+      + apply Positive_as_DT.lt_succ_diag_r.
+      + eapply Forall_impl; eauto.
+        intros [x _] Hlt'.
+        apply Positive_as_OT.lt_lt_succ; auto.
+      + intro contra.
+        induction l; inv H; simpl in *; auto.
+        destruct a as [x ann].
+        destruct contra; subst; inv H0; auto.
+        apply Pos.lt_irrefl in H3; auto.
+    Qed.
+
+    Fact fresh_ident_st_follows :
+      forall (b : B) id st st',
+        fresh_ident b st = (id, st') ->
+        fresh_st_follows st st'.
+    Proof.
+      intros b res st st' Hfresh.
+      destruct st as [n l]; destruct st' as [n' l'].
+      simpl in *; inv Hfresh; simpl.
+      unfold fresh_st_follows, smallest_ident in *; simpl in *.
+      split.
+      - apply incl_tl. reflexivity.
+      - induction l as [|[a ?]]; simpl in *.
+        + rewrite Pos.min_glb_iff.
+          split.
+          * reflexivity.
+          * apply Pos.lt_le_incl.
+            apply Pos.lt_succ_diag_r.
+        + rewrite Pos.min_glb_iff in *.
+          destruct IHl as [IHl1 IHl2].
+          split.
+          * etransitivity; eauto.
+            eapply Pos.le_min_r.
+          * eapply Pos.min_le_compat_l; eauto.
+    Qed.
+  End fresh_ident.
+
+  Section bind.
+    Context {A A' B : Type}.
+
+    Definition bind (x : Fresh A B) (k : A -> Fresh A' B) : Fresh A' B :=
+      fun st => let '(a, st') := x st in k a st'.
+
+    Lemma bind_spec : forall (x : Fresh A B) (k : A -> Fresh A' B) st a' st'',
+        (bind x k) st = (a', st'') <->
+        exists a, exists st', (x st = (a, st') /\ k a st' = (a', st'')).
+    Proof.
+      intros x k st a' st''. split; intros.
+      - unfold bind in H.
+        destruct (x st) as [a st']. exists a. exists st'.
+        split; auto.
+      - destruct H as [a [st' [H1 H2]]]. unfold bind.
+        rewrite H1. assumption.
+    Qed.
+  End bind.
+
+  Section bind2.
+    Context {A1 A2 A' B : Type}.
+
+    Definition bind2 (x: Fresh (A1 * A2) B) (k: A1 -> A2 -> Fresh A' B) : Fresh A' B :=
+      fun n => let '((a1, a2), n') := x n in k a1 a2 n'.
+
+    Lemma bind2_spec : forall (x : Fresh (A1 * A2) B) (k : A1 -> A2 -> Fresh A' B) st a' st'',
+        (bind2 x k) st = (a', st'') <->
+        exists a1, exists a2, exists st', (x st = ((a1, a2), st') /\ k a1 a2 st' = (a', st'')).
+    Proof.
+      intros x k st a' st''. split; intros.
+      - unfold bind2 in H.
+        destruct (x st) as [[a1 a2] st']. exists a1. exists a2. exists st'.
+        split; auto.
+      - destruct H as [a1 [a2 [st' [H1 H2]]]]. unfold bind2.
+        rewrite H1. assumption.
+    Qed.
+  End bind2.
+End Fresh.
+
+Section Instances.
   Context {B : Type}.
+  Global Instance st_follows_refl : Reflexive (@Fresh.fresh_st_follows B) := Fresh.st_follows_refl.
+  Global Instance st_follows_trans : Transitive (@Fresh.fresh_st_follows B) := Fresh.st_follows_trans.
+End Instances.
 
-  (** The counter is incremented with each call to `fresh_name` *)
-  Definition fresh_ident (b : B) : Fresh ident B :=
-    fun '(n, l) => (n, (Pos.succ n, (cons (n, b) l))).
+Module Facts.
+  Import Fresh.
 
-  Fact fresh_ident_st_valid :
-    forall (b : B) res st st',
-      fresh_ident b st = (res, st') ->
-      fresh_st_valid st ->
-      fresh_st_valid st'.
-  Proof.
-    intros b res st st' Hfresh Hvalid.
-    destruct st as [n l]; destruct st' as [n' l'].
-    simpl in Hfresh; inv Hfresh.
-    destruct Hvalid.
-    repeat constructor; auto.
-    + apply Positive_as_DT.lt_succ_diag_r.
-    + eapply Forall_impl; eauto.
-      intros [x _] Hlt'.
-      apply Positive_as_OT.lt_lt_succ; auto.
-    + intro contra.
-      induction l; inv H; simpl in *; auto.
-      destruct a as [x ann].
-      destruct contra; subst; inv H0; auto.
-      apply Pos.lt_irrefl in H3; auto.
-  Qed.
+  Section st.
+    Context {B : Type}.
 
-  Fact fresh_ident_st_follows :
-    forall (b : B) res st st',
-      fresh_ident b st = (res, st') ->
-      fresh_st_follows st st'.
-  Proof.
-    intros b res st st' Hfresh.
-    destruct st as [n l]; destruct st' as [n' l'].
-    simpl in *; inv Hfresh; simpl.
-    unfold fresh_st_follows, smallest_ident in *; simpl in *.
-    split.
-    - apply incl_tl. reflexivity.
-    - induction l as [|[a ?]]; simpl in *.
-      + rewrite Pos.min_glb_iff.
-        split.
-        * reflexivity.
-        * apply Pos.lt_le_incl.
-          apply Pos.lt_succ_diag_r.
-      + rewrite Pos.min_glb_iff in *.
-        destruct IHl as [IHl1 IHl2].
-        split.
-        * etransitivity; eauto.
-          eapply Pos.le_min_r.
-        * eapply Pos.min_le_compat_l; eauto.
-  Qed.
+    Fact st_anns_ids_In : forall (st : fresh_st B) id,
+        (exists b, In (id, b) (st_anns st)) <-> In id (st_ids st).
+    Proof.
+      intros.
+      split; intros.
+      - destruct H as [b H].
+        unfold st_ids. rewrite in_map_iff.
+        exists (id, b); auto.
+      - unfold st_ids in H. rewrite in_map_iff in H.
+        destruct H as [[? b] [? H]]; simpl in *; subst.
+        exists b. assumption.
+    Qed.
+  End st.
 
-  Fact fresh_ident_vars_perm : forall (b : B) id st st',
-      fresh_ident b st = (id, st') ->
-      Permutation (id::(map fst (snd st))) (map fst (snd st')).
-  Proof.
-    intros b id st st' Hfresh.
-    destruct st; destruct st'; simpl in *.
-    inv Hfresh. simpl. reflexivity.
-  Qed.
-End fresh_ident.
+  Section fresh_ident.
+    Context {B : Type}.
 
-Section bind.
-  Context {A A' B : Type}.
+    Fact fresh_ident_In : forall (b : B) id st st',
+        fresh_ident b st = (id, st') ->
+        In (id, b) (st_anns st').
+    Proof.
+      intros. apply fresh_ident_anns in H.
+      rewrite H. constructor. reflexivity.
+    Qed.
 
-  Definition bind (x : Fresh A B) (k : A -> Fresh A' B) : Fresh A' B :=
-    fun st => let '(a, st') := x st in k a st'.
+    Fact fresh_ident_vars_perm : forall (b : B) id st st',
+        fresh_ident b st = (id, st') ->
+        Permutation (id::(st_ids st)) (st_ids st').
+    Proof.
+      intros. apply fresh_ident_anns in H.
+      unfold st_ids in *. rewrite H.
+      reflexivity.
+    Qed.
+  End fresh_ident.
+End Facts.
 
-  Lemma bind_inv : forall (x : Fresh A B) (k : A -> Fresh A' B) st a' st'',
-      (bind x k) st = (a', st'') ->
-      exists a, exists st', (x st = (a, st') /\ k a st' = (a', st'')).
-  Proof.
-    intros x k st a' st'' Hbind.
-    unfold bind in Hbind.
-    destruct (x st) as [a st']. exists a. exists st'.
-    split; auto.
-  Qed.
-End bind.
+Module Tactics.
+  Import Fresh.
+  Ltac inv_bind :=
+    match goal with
+    | H : context c [ret _ _] |- _ =>
+      rewrite ret_spec in H
+    | H : (_, _) = (_, _) |- _ =>
+      inv H
+    | H : bind _ _ _ = (_, _) |- _ =>
+      apply bind_spec in H; destruct H as [? [? [? ?]]]; simpl
+    | H : bind2 _ _ _ = (_, _) |- _ =>
+      apply bind2_spec in H; destruct H as [? [? [? [? ?]]]]; simpl
+    | |- context c [ret _ _] =>
+      rewrite ret_spec
+    | |- bind _ _ _ = (_, _) =>
+      rewrite bind_spec
+    | |- bind2 _ _ _ = (_, _) =>
+      rewrite bind2_spec
+    end.
+End Tactics.
 
-Section bind2.
-  Context {A1 A2 A' B : Type}.
+Module Notations.
+  Import Fresh.
+  (** [do] notation, inspired by CompCert's error monad *)
+  Notation "'do' X <- A ; B" :=
+    (bind A (fun X => B))
+      (at level 200, X ident, A at level 100, B at level 200): fresh_monad_scope.
 
-  Definition bind2 (x: Fresh (A1 * A2) B) (k: A1 -> A2 -> Fresh A' B) : Fresh A' B :=
-    fun n => let '((a1, a2), n') := x n in k a1 a2 n'.
-
-  Lemma bind2_inv : forall (x : Fresh (A1 * A2) B) (k : A1 -> A2 -> Fresh A' B) st a' st'',
-      (bind2 x k) st = (a', st'') ->
-      exists a1, exists a2, exists st', (x st = ((a1, a2), st') /\ k a1 a2 st' = (a', st'')).
-  Proof.
-    intros x k st a' st'' Hbind.
-    unfold bind2 in Hbind.
-    destruct (x st) as [[a1 a2] st']. exists a1. exists a2. exists st'.
-    split; auto.
-  Qed.
-End bind2.
-
-Ltac inv_bind :=
-  match goal with
-  | H : ret _ _ = _ |- ?G =>
-    unfold ret in H; inv H; simpl
-  | H : bind _ _ _ = (_, _) |- _ =>
-    apply bind_inv in H; destruct H as [? [? [? ?]]]; simpl
-  | H : bind2 _ _ _ = (_, _) |- _ =>
-    apply bind2_inv in H; destruct H as [? [? [? [? ?]]]]; simpl
-  | |- ret _ _ = _ =>
-    unfold ret; simpl
-  | |- bind _ _ _ = (_, _) =>
-    unfold bind; simpl
-  | |- bind2 _ _ _ = (_, _, _) =>
-    unfold bind2; simpl
-  end.
-
-(** [do] notation, inspired by CompCert's error monad *)
-Notation "'do' X <- A ; B" :=
-  (bind A (fun X => B))
-    (at level 200, X ident, A at level 100, B at level 200): fresh_monad_scope.
-
-Notation "'do' ( X , Y ) <- A ; B" :=
-  (bind2 A (fun X Y => B))
-    (at level 200, X ident, Y ident, A at level 100, B at level 200): fresh_monad_scope.
+  Notation "'do' ( X , Y ) <- A ; B" :=
+    (bind2 A (fun X Y => B))
+      (at level 200, X ident, Y ident, A at level 100, B at level 200): fresh_monad_scope.
+End Notations.
 
 Section map_bind2.
+  Import Fresh Tactics Notations.
+  Open Scope fresh_monad_scope.
   Context {A A1 A2 B : Type}.
   Variable k : A -> Fresh (A1 * A2) B.
 
-  Open Scope list.
-  Open Scope fresh_monad_scope.
   Fixpoint map_bind2 a :=
     match a with
     | nil => ret (nil, nil)
     | hd::tl => do (a1, a2) <- k hd;
-                do (a1s, a2s) <- map_bind2 tl;
-                ret (a1::a1s, a2::a2s)
+              do (a1s, a2s) <- map_bind2 tl;
+              ret (a1::a1s, a2::a2s)
     end.
 
   Fact map_bind2_values : forall a st a1s a2s st',
       map_bind2 a st = (a1s, a2s, st') ->
       Forall3 (fun a a1 a2 => exists st'', exists st''', k a st'' = (a1, a2, st''')) a a1s a2s.
   Proof.
-    induction a; intros st a1s a2s st' Hfold; simpl in *.
-    - inv Hfold. constructor.
-    - repeat inv_bind.
-      specialize (IHa _ _ _ _ H0).
+    induction a; intros st a1s a2s st' Hfold; simpl in *; repeat inv_bind.
+    - constructor.
+    - specialize (IHa _ _ _ _ H0).
       constructor; eauto.
   Qed.
 
@@ -226,7 +453,8 @@ Section map_bind2.
   Qed.
 End map_bind2.
 
-Hint Resolve fresh_ident_st_follows.
-Hint Resolve fresh_ident_st_valid.
+Hint Resolve Fresh.st_follows_smallest.
+Hint Resolve Fresh.fresh_ident_st_follows.
+Hint Resolve Fresh.fresh_ident_st_valid.
 Hint Resolve map_bind2_st_valid.
 Hint Resolve map_bind2_st_follows.
